AExp.thy
@@ -1,20 +1,9 @@
-section\<open>Extended Finite State Machines\<close>
+section \<open>Arithmetic Expressions\<close>
 text\<open>
-This section presents the theories associated with EFSMs. First we define a language of arithmetic
-expressions for guards, outputs, and updates similar to that in IMP \cite{fixme}. We then go on to
-define the guard logic such that nonsensical guards (such as testing to see if an integer is greater
-than a string) can never evaluate to true. Next, the guard language is defined in terms of
-arithmetic expressions and binary relations. In the interest of simplifying the conversion of guards
-to constraints, we use a Nor logic, although we define syntax hacks for the expression of guards
-using other logical operators. With the underlying types defined, we then define EFSMs and prove
-that they are prefix-closed, that is to say that if a string of inputs is accepted by the machine
-then all of its prefixes are also accepted.
-\<close>
-subsection \<open>Arithmetic Expressions\<close>
-text\<open>
-This theory defines a language of arithmetic expressions over literal values and variables. Here,
+This theory defines a language of arithmetic expressions over variables and literal values. Here,
 values are limited to integers and strings. Variables may be either inputs or registers. We also
-limit ourselves to a simple arithmetic of plus and minus as a proof of concept.
+limit ourselves to a simple arithmetic of addition, subtraction, and multiplication as a proof of
+concept.
 \<close>
 
 theory AExp
