GExp.thy
@@ -1,14 +1,14 @@
 subsection \<open>Guards Expressions\<close>
 text\<open>
 This theory defines the guard language of EFSMs which can be translated directly to and from
-contexts. This is similar to boolean expressions from IMP \cite{fixme}. Boolean values true and
-false respectively represent the guards which are always and never satisfied. Guardss may test
-for (in)equivalence of two arithmetic expressions or be connected using nor logic into compound
-expressions. Additionally, a guard may also test to see if a particular variable is null. This is
-useful if an EFSM transition is intended only to initialise a register.  We also define syntax hacks
-for the relations less than, less than or equal to, greater than or equal to, and not equal to as
-well as the expression of logical conjunction, disjunction, and negation in terms of nor logic.
-\<close>
+contexts. Boolean values true and false respectively represent the guards which are always and never
+satisfied. Guards may test for (in)equivalence of two arithmetic expressions or be connected using
+\textsc{nor} logic into compound expressions. The use of \textsc{nor} logic reduces the number of
+subgoals when inducting over guard expressions.
+
+We also define syntax hacks for the relations less than, less than or equal to, greater than or
+equal to, and not equal to as well as the expression of logical conjunction, disjunction, and
+negation in terms of nor logic.\<close>
 
 theory GExp
 imports AExp Trilean
